Make BoogieV executable (#2)
This PR makes BoogieV executable and fixes some other related issues.

Some of the main changes that were made in order to get to this point are:

- Forall and exists quantifiers have been commented out (to not have to worry about binders)
- Added generation of VC. The VC is then handed to an SMT solver. The connection to the SMT solver is implemented by using the prover interface in Boogie 2.
- Let expressions are introduced to generate the VC (but for now let expressions are not supported before the generation of the VC, so binders do not appear before the VC)
- Pretty printer is now expressed as a function instead of as method.
- Added elimination of if guards and a corresponding proof.
- There was a bug in the loop elimination (loops were not eliminated recursively). This bug was fixed and the lemma was strengthened accordingly (postcondition ensures that resulting program indeed has no loops).
- A merge sort implemented by Rustan Leino is used to convert a set to a sequence.

smt_interface/csharp_smt_interface/Program.cs
@@ -1,0 +1,236 @@
+﻿using Microsoft.Boogie.VCExprAST;
+using Microsoft.Boogie;
+using Microsoft.Boogie.SMTLib;
+using Dafny;
+
+namespace SMTInterface_Compile
+{
+    public class VCExprInterface
+    {
+        private VCExpressionGenerator exprGen;
+        private string proverPath;
+        private string logPath;
+
+        ProverFactory proverFactory = ProverFactory.Load("SMTLib");
+
+        /* keep a map from strings to var objects to make sure that we can return
+        the same object for the same name (on the Dafny side variables are different
+        iff their names are different) */
+        private IDictionary<string, VCExprVar> nameToVar = new Dictionary<string, VCExprVar>();
+
+        public VCExprInterface(VCExpressionGenerator exprGen, string proverPath, string logPath)
+        {
+            this.exprGen = exprGen;
+            this.proverPath = proverPath;
+            this.logPath = logPath;
+        }
+        
+        public static VCExprInterface Create(ISequence<char> proverPath, ISequence<char> logPath)
+        {
+          var exprGen = new VCExpressionGenerator();
+          return new VCExprInterface(exprGen, proverPath.ToString(), logPath.ToString());
+        }
+
+        private async Task<ProverInterface.Outcome> InvokeProver(ProverInterface proverInterface, VCExpr vc, ProverInterface.ErrorHandler errorHandler, int errorLimit)
+        {
+          var proverOutcomeTask = 
+            proverInterface.Check(
+              "vc_query",
+              vc,
+              errorHandler,
+              errorLimit,
+              CancellationToken.None
+            );
+
+          var outcome = await proverOutcomeTask;
+          return outcome;
+        }
+
+        public bool IsVCValid(VCExpr vc)
+        {
+          var options = CommandLineOptions.FromArguments();
+          options.SIBoolControlVC = true;
+          var proverOptions = (SMTLibSolverOptions) proverFactory.BlankProverOptions(options);
+          proverOptions.Parse(new List<string> { 
+            "PROVER_PATH="+proverPath,
+            "LOG_FILE="+logPath
+            });
+          var proverContext = proverFactory.NewProverContext(proverOptions);
+          ProverInterface proverInterface = 
+            proverFactory.SpawnProver(
+              options, 
+              proverOptions, 
+              proverContext
+            );
+          
+          var proverOutcome = 
+            InvokeProver(
+              proverInterface,
+              vc,
+              new ProverInterface.ErrorHandler(options),
+              options.ErrorLimit
+            ).Result;
+
+          //TODO give information on other outcomes
+          return proverOutcome == ProverInterface.Outcome.Valid;
+        }
+
+        public VCExpr VCIntVar(Dafny.ISequence<char> x) 
+        {
+            string xS = x.ToString();
+            if(!nameToVar.TryGetValue(xS, out var res)) {
+                var intType = Microsoft.Boogie.Type.Int;
+                res = exprGen.Variable(xS, intType);
+                nameToVar.Add(xS, res);
+            }
+
+            return res;
+        }
+
+        public VCExpr VCBoolVar(Dafny.ISequence<char> x) 
+        {
+            string xS = x.ToString();
+            if(!nameToVar.TryGetValue(xS, out var res)) {
+                var boolType = Microsoft.Boogie.Type.Bool;
+                res = exprGen.Variable(xS, boolType);
+                nameToVar.Add(xS, res);
+            }
+
+            return res;
+        }
+
+        public VCExpr VCLitInt(System.Numerics.BigInteger i) 
+        {
+            return exprGen.Integer(Microsoft.BaseTypes.BigNum.FromBigInt(i));
+        }
+
+        public VCExpr VCLitBool(bool b) 
+        {
+            if(b) {
+                return VCExpressionGenerator.True;
+            } else {
+                return VCExpressionGenerator.False;
+            }
+        }
+
+        public VCExpr VCEq(VCExpr e1, VCExpr e2)
+        {
+          return exprGen.Function(VCExpressionGenerator.EqOp, e1, e2);
+        }
+
+        public VCExpr VCNeq(VCExpr e1, VCExpr e2)
+        {
+          return exprGen.Function(VCExpressionGenerator.NeqOp, e1, e2);
+        }
+
+        public VCExpr VCAdd(VCExpr e1, VCExpr e2)
+        {
+          return exprGen.Function(VCExpressionGenerator.AddIOp, e1, e2);
+        }
+
+        public VCExpr VCSub(VCExpr e1, VCExpr e2)
+        {
+          return exprGen.Function(VCExpressionGenerator.SubIOp, e1, e2);
+        }
+
+        public VCExpr VCMul(VCExpr e1, VCExpr e2)
+        {
+          return exprGen.Function(VCExpressionGenerator.MulIOp, e1, e2);
+        }
+
+        public VCExpr VCDiv(VCExpr e1, VCExpr e2)
+        {
+          return exprGen.Function(VCExpressionGenerator.DivIOp, e1, e2);
+        }
+
+        public VCExpr VCMod(VCExpr e1, VCExpr e2)
+        {
+          return exprGen.Function(VCExpressionGenerator.ModOp, e1, e2);
+        }
+
+        public VCExpr VCLt(VCExpr e1, VCExpr e2)
+        {
+          return exprGen.Function(VCExpressionGenerator.LtOp, e1, e2);
+        }
+
+        public VCExpr VCLe(VCExpr e1, VCExpr e2)
+        {
+          return exprGen.Function(VCExpressionGenerator.LeOp, e1, e2);
+        }
+
+        public VCExpr VCGt(VCExpr e1, VCExpr e2)
+        {
+          return exprGen.Function(VCExpressionGenerator.GtOp, e1, e2);
+        }
+
+        public VCExpr VCGe(VCExpr e1, VCExpr e2)
+        {
+          return exprGen.Function(VCExpressionGenerator.GeOp, e1, e2);
+        }
+
+        public VCExpr VCAnd(VCExpr e1, VCExpr e2)
+        {
+          return exprGen.Function(VCExpressionGenerator.AndOp, e1, e2);
+        }
+
+        public VCExpr VCOr(VCExpr e1, VCExpr e2)
+        {
+          return exprGen.Function(VCExpressionGenerator.OrOp, e1, e2);
+        }
+
+        public VCExpr VCImp(VCExpr e1, VCExpr e2)
+        {
+          return exprGen.Function(VCExpressionGenerator.ImpliesOp, e1, e2);
+        }
+        
+        public VCExpr VCIff(VCExpr e1, VCExpr e2)
+        {
+          //same as Eq (also the case in the Boogie 2 implementation at this point)
+          return exprGen.Function(VCExpressionGenerator.EqOp, e1, e2);
+        }
+
+        public VCExpr VCNot(VCExpr e)
+        {
+            return exprGen.Function(VCExpressionGenerator.NotOp, e);
+        }
+
+        public VCExpr VCUMinus(VCExpr e)
+        {
+          //there is no unary minus in VCExpr --> Boogie 2 does the same encoding
+          return exprGen.Function(VCExpressionGenerator.SubIOp, exprGen.Integer(Microsoft.BaseTypes.BigNum.ZERO), e);
+        }
+
+        public VCExpr VCLet(Dafny.ISequence<char> varName, VCExpr binding, VCExpr body)
+        {
+          //we only support boolean variables
+          var vcExprVar = (VCExprVar) VCBoolVar(varName);
+          var letBinding = exprGen.LetBinding(vcExprVar, binding);
+          return exprGen.Let(new List<VCExprLetBinding> { letBinding }, body);
+        }
+
+    }
+
+    class MainClass {
+      static void Main(string [] args) {
+        if(args.Length < 2) {
+          Console.WriteLine("Not enough arguments (need at least two)");
+          return;
+        }
+
+        var vcExprGen = new VCExpressionGenerator();
+        var exprInterface = new VCExprInterface(vcExprGen, args[0], args[1]);
+
+        var x = vcExprGen.Variable("test", Microsoft.Boogie.Type.Int);
+
+        var vc = 
+          vcExprGen.Implies(vcExprGen.Gt(x, exprInterface.VCLitInt(4)), vcExprGen.Gt(x, exprInterface.VCLitInt(2)));
+
+        var isVCValid = exprInterface.IsVCValid(vc);
+        if(isVCValid) {
+          Console.Out.WriteLine("Input program is correct.");
+        } else {
+          Console.Out.WriteLine("Input program might not be correct.");
+        }
+      }
+    }
+}
