transformations/DesugarScopedVarsImpl.dfy
@@ -2,6 +2,7 @@ include "../lang/BoogieSemantics.dfy"
 include "../dafny-libraries/src/Collections/Sequences/Seq.dfy"
 include "../dafny-libraries/src/Collections/Maps/Maps.dfy"
 include "../util/Naming.dfy"
+include "../util/AstSubsetPredicates.dfy"
 
 module DesugarScopedVarsImpl {
 
@@ -12,6 +13,7 @@ module DesugarScopedVarsImpl {
   import Util
   import opened Wrappers
   import opened Naming
+  import opened AstSubsetPredicates
 
   function method CreateUniqueVarDecls(varDecls: seq<(var_name, Ty)>, counter: nat) : seq<(var_name,Ty)>
     ensures 
@@ -110,9 +112,9 @@ module DesugarScopedVarsImpl {
       var (els', counter'') := MakeScopedVarsUnique(els, substMap, counter');
       (If(None, thn', els'), counter'')
     case _ => (c, counter) //TODO (precondition should eliminate this case)
-  }  
- 
-  function method RemoveScopedVars(c: Cmd): (Cmd, (seq<(var_name, Ty)>))
+  }   
+
+  function method RemoveScopedVarsAux(c: Cmd): (Cmd, seq<VarDecl>)
     /*requires substMap.Values <= set c,x | x in substMap.Keys && 0 < c < usedVars.1 :: VersionedName(x, c)
     requires forall x | x in substMap.Keys :: exists c : nat :: c <= usedVars.1 && substMap[x] == VersionedName(x, c)
     ensures 
@@ -122,18 +124,46 @@ module DesugarScopedVarsImpl {
     case SimpleCmd(sc) => (c, [])
     case Break(_) => (c, [])
     case Seq(c1, c2) => 
-      var (c1', decls1) := RemoveScopedVars(c1);
-      var (c2', decls2) := RemoveScopedVars(c2);
+      var (c1', decls1) := RemoveScopedVarsAux(c1);
+      var (c2', decls2) := RemoveScopedVarsAux(c2);
       (Seq(c1', c2'), decls1 + decls2)
     case Scope(optLabel, varDecls, body) =>
-      var (body', declsBody) := RemoveScopedVars(body);
+      var (body', declsBody) := RemoveScopedVarsAux(body);
       (Scope(optLabel, [], body'), varDecls + declsBody)
     case If(None, thn, els) => 
       //TODO: make sure If(Some(...)) has been desugared
-      var (thn', declsThn) := RemoveScopedVars(thn);
-      var (els', declsEls) := RemoveScopedVars(els);
+      var (thn', declsThn) := RemoveScopedVarsAux(thn);
+      var (els', declsEls) := RemoveScopedVarsAux(els);
       (If(None, thn', els'), declsThn + declsEls)
     case _ => (c, []) //TODO (precondition should eliminate this case)
+  }
+
+  function method RemoveScopedVars(c: Cmd) : (Cmd, seq<VarDecl>)
+  {
+    var (cUnique, _) := MakeScopedVarsUnique(c, map[], 0);
+    var (c', decls) := RemoveScopedVarsAux(cUnique);
+    (c', decls)
+  }
+
+  lemma MakeScopedVarsUniquePreserveStructure(c: Cmd, substMap: map<var_name, var_name>, counter: nat)
+    requires NoLoopsNoIfGuard(c) && NoBreaks(c)
+    ensures 
+      var (c', _) := MakeScopedVarsUnique(c, substMap, counter);
+      NoLoopsNoIfGuard(c') && NoBreaks(c')
+  { }
+
+  lemma RemoveScopedVarsAuxPreserveStructure(c: Cmd)
+    requires NoLoopsNoIfGuard(c) && NoBreaks(c)
+    ensures NoLoopsNoIfGuardNoScopedVars(RemoveScopedVarsAux(c).0) && NoBreaks(RemoveScopedVarsAux(c).0)
+  { }
+
+  lemma RemoveScopedVarsStructure(c: Cmd)
+    requires NoLoopsNoIfGuard(c) && NoBreaks(c)
+    ensures NoLoopsNoIfGuardNoScopedVars(RemoveScopedVars(c).0) && NoBreaks(RemoveScopedVars(c).0)
+  { 
+    var (cUnique, _) := MakeScopedVarsUnique(c, map[], 0);
+    MakeScopedVarsUniquePreserveStructure(c, map[], 0);
+    RemoveScopedVarsAuxPreserveStructure(cUnique);
   }
 
   function GetDecls(c: Cmd) : seq<VarDecl>
@@ -157,13 +187,13 @@ module DesugarScopedVarsImpl {
   }
 
   /** TODO */
+  /*
   lemma UniqueVars(c: Cmd, substMap: map<var_name, var_name>, counter: nat)
     ensures 
       var (c', counter') := MakeScopedVarsUnique(c, substMap, counter);
       && Sequences.HasNoDuplicates(GetDecls(c'))
       && counter <= counter'
   { assume false; }
-  
-
+  */
 
 }
