transformations/LoopElim.dfy
@@ -1,78 +1,231 @@
 include "../lang/BoogieLang.dfy"
 include "../lang/BoogieSemantics.dfy"
+include "../util/AstSubsetPredicates.dfy"
 include "../dafny-libraries/src/Wrappers.dfy"
 
-import opened BoogieLang
-import opened BoogieSemantics
-import opened Wrappers
+
+module LoopElim {
+    import opened BoogieLang
+    import opened BoogieSemantics
+    import opened Wrappers
+    import opened AstSubsetPredicates
 
 
-function EliminateLoops(c: Cmd) : Cmd {
-    match c
-    case Scope(optLbl, varDecls, body) => Scope(optLbl, varDecls, EliminateLoops(body))
-    case If(optCond, thn, els) => If(optCond, EliminateLoops(thn), EliminateLoops(els))
-    case Loop(invs, body) =>
+    lemma LabelsWellDefSeqToCmd(cs: seq<Cmd>, lbls: set<lbl_name>)
+    requires |cs| > 0
+    requires LabelsWellDefAux(SeqToCmd(cs), lbls)
+    ensures forall i | 0 <= i < |cs| :: LabelsWellDefAux(cs[i], lbls)
+    {
+        if |cs| == 1 {
+        } else {
+            var cs' := cs[1..];
+            LabelsWellDefSeqToCmd(cs', lbls);
+        }
+    }
+
+    lemma WpSeqToCmdSingleDiff<A(!new)>(a: absval_interp<A>, cs1: seq<Cmd>, cs2: seq<Cmd>, diffIdx: nat, post: WpPost<A>, s: state<A>)
+        requires |cs1| == |cs2|
+        requires 0 <= diffIdx < |cs1|
+        requires forall i | 0 <= i < |cs1| && i != diffIdx :: cs1[i] == cs2[i] 
+        requires LabelsWellDefAux(SeqToCmd(cs1), post.scopes.Keys)
+        requires LabelsWellDefAux(SeqToCmd(cs2), post.scopes.Keys)
+        requires forall s, post':WpPost<A> | post'.scopes.Keys == post.scopes.Keys :: 
+            (LabelsWellDefSeqToCmd(cs1, post.scopes.Keys);
+            LabelsWellDefSeqToCmd(cs2, post.scopes.Keys);
+            WpCmd(a, cs1[diffIdx], post')(s) == WpCmd(a, cs2[diffIdx], post')(s))
+        
+        ensures WpCmd(a, SeqToCmd(cs1), post)(s) == WpCmd(a, SeqToCmd(cs2), post)(s)
+    {
+        reveal WpCmd(); //need this due to opaque bug (otherwise cannot use the quantifier in the precondition)
+
+        if |cs1| == 1 {
+
+        } else {
+            calc {
+                WpCmd(a, SeqToCmd(cs1), post)(s);
+                WpCmd(a, Seq(cs1[0], SeqToCmd(cs1[1..])), post)(s);
+                WpCmd(a, cs1[0], WpPost(WpCmd(a, SeqToCmd(cs1[1..]), post), post.currentScope, post.scopes))(s);
+                {  
+                    forall s' | true 
+                    ensures WpCmd(a, SeqToCmd(cs1[1..]), post)(s') == WpCmd(a, SeqToCmd(cs2[1..]), post)(s')
+                    {
+                        if diffIdx != 0 {
+                            WpSeqToCmdSingleDiff(a, cs1[1..], cs2[1..], diffIdx-1, post, s');
+                        } else {
+                            assert cs1[1..] == cs2[1..];
+                        }
+                    }
+
+                    WpCmdPointwise(a, cs1[0], WpPost(WpCmd(a, SeqToCmd(cs1[1..]), post), post.currentScope, post.scopes), 
+                                              WpPost(WpCmd(a, SeqToCmd(cs2[1..]), post), post.currentScope, post.scopes), s);
+                }
+                WpCmd(a, cs2[0], WpPost(WpCmd(a, SeqToCmd(cs2[1..]), post), post.currentScope, post.scopes))(s);
+                WpCmd(a, Seq(cs2[0], SeqToCmd(cs2[1..])), post)(s);
+            }
+        }
+    }
+
+    lemma PredicateRecSeqToCmd(cs: seq<Cmd>, predCmd: Cmd -> bool, predSimpleCmd: SimpleCmd -> bool, predExpr: Expr -> bool)
+      requires |cs| > 0
+      requires forall c : Cmd | c.Seq? :: predCmd(c)
+      requires forall c | c in cs :: c.PredicateRec(predCmd, predSimpleCmd, predExpr)
+      ensures SeqToCmd(cs).PredicateRec(predCmd, predSimpleCmd, predExpr)
+    { 
+        if |cs| > 1 {
+          calc {
+            SeqToCmd(cs).PredicateRec(predCmd, predSimpleCmd, predExpr);
+            Seq(cs[0], SeqToCmd(cs[1..])).PredicateRec(predCmd, predSimpleCmd, predExpr);
+            && cs[0].PredicateRec(predCmd, predSimpleCmd, predExpr)
+            && SeqToCmd(cs[1..]).PredicateRec(predCmd, predSimpleCmd, predExpr);
+          }
+        }
+    }
+
+    /** TODO: the following two lemmas should be derived from a more general lemma on Cmd.PredicatRec */
+    lemma NoBreaksSeqToCmd(cs: seq<Cmd>)
+      requires |cs| > 0
+      requires forall c | c in cs :: NoBreaks(c);
+      ensures NoBreaks(SeqToCmd(cs))
+    { 
+        PredicateRecSeqToCmd(cs, (cmd: Cmd) => !cmd.Break?, sc => true, e => true);
+    }
+    
+    lemma NoLoopsSeqToCmd(cs: seq<Cmd>)
+      requires |cs| > 0
+      requires forall c | c in cs :: NoLoops(c);
+      ensures NoLoops(SeqToCmd(cs))
+    { 
+        PredicateRecSeqToCmd(cs, (cmd: Cmd) => !cmd.Loop?, sc => true, e => true);
+    }
+
+    function method EliminateLoops(c: Cmd) : Cmd 
+    ensures NoLoops(EliminateLoops(c))
+    {
+        match c
+        case Scope(optLbl, varDecls, body) => Scope(optLbl, varDecls, EliminateLoops(body))
+        case If(optCond, thn, els) => If(optCond, EliminateLoops(thn), EliminateLoops(els))
+        case Loop(invs, body) =>
+            var modDecls : seq<(var_name, Ty)> := ModifiedVars(body);
+            var invsConj := NAryBinOp(And, Expr.TrueExpr, invs);
+            var body' := EliminateLoops(body);
+
+            var seqResult :=
+                [ SimpleCmd(Assert(invsConj)),
+                SimpleCmd(Havoc(modDecls)),
+                SimpleCmd(Assume(invsConj)),
+                body',
+                SimpleCmd(Assert(invsConj)),
+                SimpleCmd(Assume(Expr.FalseExpr))
+                ];
+            
+            assert NoLoops(body');
+            NoLoopsSeqToCmd(seqResult);
+            
+            SeqToCmd(seqResult)
+        case Seq(c1, c2) =>
+            Seq(EliminateLoops(c1), EliminateLoops(c2))
+        case _ => c
+    }
+
+    lemma EliminateLoopsPreserveNoBreaks(c: Cmd)
+    requires NoBreaks(c)
+    ensures NoBreaks(EliminateLoops(c))
+    {
+      match c
+      case Loop(invs, body) =>
         var modDecls : seq<(var_name, Ty)> := ModifiedVars(body);
         var invsConj := NAryBinOp(And, Expr.TrueExpr, invs);
+        var body' := EliminateLoops(body);
 
         var seqResult :=
             [ SimpleCmd(Assert(invsConj)),
-              SimpleCmd(Havoc(modDecls)),
-              SimpleCmd(Assume(invsConj)),
-              body,
-              SimpleCmd(Assert(invsConj)),
-              SimpleCmd(Assume(Expr.FalseExpr))
+            SimpleCmd(Havoc(modDecls)),
+            SimpleCmd(Assume(invsConj)),
+            body',
+            SimpleCmd(Assert(invsConj)),
+            SimpleCmd(Assume(Expr.FalseExpr))
             ];
         
-        SeqToCmd(seqResult)
-    case Seq(c1, c2) =>
-        Seq(EliminateLoops(c1), EliminateLoops(c2))
-    case _ => c
-}
+        assert NoBreaks(body');
+        NoBreaksSeqToCmd(seqResult);
+      case _ => 
+    }
 
-lemma EliminateLoopsCorrect<A(!new)>(a: absval_interp<A>, c: Cmd, s: state<A>, post: WpPost)
-requires LabelsWellDefAux(c, post.scopes.Keys) && LabelsWellDefAux(EliminateLoops(c), post.scopes.Keys)
-ensures  WpCmd(a, EliminateLoops(c), post)(s) == WpCmd(a, c, post)(s)
-{
-    reveal WpCmd();
-    match c
-    case Seq(c1, c2) => 
-        var c2Post := WpCmd(a, c2, post);
-        var c2ElimPost := WpCmd(a, EliminateLoops(c2), post);
+    lemma EliminateLoopsCorrect<A(!new)>(a: absval_interp<A>, c: Cmd, s: state<A>, post: WpPost)
+    requires LabelsWellDefAux(c, post.scopes.Keys) && LabelsWellDefAux(EliminateLoops(c), post.scopes.Keys)
+    ensures  WpCmd(a, EliminateLoops(c), post)(s) == WpCmd(a, c, post)(s)
+    {
+        reveal WpCmd();
+        match c
+        case Seq(c1, c2) => 
+            var c2Post := WpCmd(a, c2, post);
+            var c2ElimPost := WpCmd(a, EliminateLoops(c2), post);
 
-        forall s':state<A> | true
-            ensures c2ElimPost(s') == c2Post(s')
-        {
-            EliminateLoopsCorrect(a, c2, s', post);
-        }
-
-        calc {
-            WpCmd(a, EliminateLoops(c), post)(s);
-            WpCmd(a, c1, WpPost(c2ElimPost, post.currentScope, post.scopes))(s); 
-            { 
-                WpCmdPointwise(a, c1, WpPost(c2ElimPost, post.currentScope, post.scopes), WpPost(c2Post, post.currentScope, post.scopes), s);
+            forall s':state<A> | true
+                ensures c2ElimPost(s') == c2Post(s')
+            {
+                EliminateLoopsCorrect(a, c2, s', post);
             }
-            WpCmd(a, c1, WpPost(c2Post, post.currentScope, post.scopes))(s);
-        }
-    case Scope(optLabel, varDecls, body) => 
-      var updatedScopes := if optLabel.Some? then post.scopes[optLabel.value := post.normal] else post.scopes;
-      assert updatedScopes.Keys == if optLabel.Some? then {optLabel.value} + post.scopes.Keys else post.scopes.Keys;
 
-      var bodyPost := ResetVarsPost(varDecls, WpPost(post.normal, post.normal, updatedScopes), s);
+            calc {
+                WpCmd(a, EliminateLoops(c), post)(s);
+                WpCmd(a, c1, WpPost(c2ElimPost, post.currentScope, post.scopes))(s); 
+                { 
+                    WpCmdPointwise(a, c1, WpPost(c2ElimPost, post.currentScope, post.scopes), WpPost(c2Post, post.currentScope, post.scopes), s);
+                }
+                WpCmd(a, c1, WpPost(c2Post, post.currentScope, post.scopes))(s);
+            }
+        case Scope(optLabel, varDecls, body) => 
+            var updatedScopes := if optLabel.Some? then post.scopes[optLabel.value := post.normal] else post.scopes;
+            assert updatedScopes.Keys == if optLabel.Some? then {optLabel.value} + post.scopes.Keys else post.scopes.Keys;
 
-      forall s: state<A> | true 
-        ensures WpCmd(a, EliminateLoops(body), bodyPost)(s) == 
-                WpCmd(a, body, bodyPost)(s)
-      {
-          calc {
-            WpCmd(a, EliminateLoops(body), bodyPost)(s); {EliminateLoopsCorrect(a, body, s, bodyPost); }
-            WpCmd(a, body, bodyPost)(s);
-          }
-      }
+            var bodyPost := ResetVarsPost(varDecls, WpPost(post.normal, post.normal, updatedScopes), s);
 
-      ForallVarDeclsPointwise(a, varDecls, WpCmd(a, EliminateLoops(body), bodyPost), WpCmd(a, body, bodyPost), s);
-    case Loop(invs, body) =>
-        //trivial because of how the Wp is defined
+            forall s: state<A> | true 
+                ensures WpCmd(a, EliminateLoops(body), bodyPost)(s) == 
+                        WpCmd(a, body, bodyPost)(s)
+            {
+                calc {
+                    WpCmd(a, EliminateLoops(body), bodyPost)(s); {EliminateLoopsCorrect(a, body, s, bodyPost); }
+                    WpCmd(a, body, bodyPost)(s);
+                }
+            }
+            ForallVarDeclsPointwise(a, varDecls, WpCmd(a, EliminateLoops(body), bodyPost), WpCmd(a, body, bodyPost), s);
+        case Loop(invs, body) =>
+            LoopDesugaringNumScopesAndLoops(invs, body);
+            LoopDesugaringLabelsWellDef(invs, body, post.scopes.Keys);
 
-    case _ => //trivial (EliminateLoops is the identity function here)
+            var body' := EliminateLoops(body);
+
+            var loopTargets := ModifiedVars(body);
+            var invsConj := NAryBinOp(And, Expr.TrueExpr, invs);
+
+            var desugaredLoop := body' => [SimpleCmd(Assert(invsConj)), SimpleCmd(Havoc(loopTargets)), SimpleCmd(Assume(invsConj)), body',  SimpleCmd(Assert(invsConj)), SimpleCmd(Assume(Expr.FalseExpr))];
+
+            assert LabelsWellDefAux(SeqToCmd(desugaredLoop(body)), post.scopes.Keys);
+            assert LabelsWellDefAux(SeqToCmd(desugaredLoop(body')), post.scopes.Keys);
+
+            forall s', post' : WpPost<A> | post'.scopes.Keys == post.scopes.Keys
+            ensures WpCmd(a, body, post')(s') == WpCmd(a, body', post')(s')
+            {
+              assert LabelsWellDefAux(body, post.scopes.Keys) by {
+                assert desugaredLoop(body)[3] == body;
+                LabelsWellDefSeqToCmd(desugaredLoop(body), post.scopes.Keys);
+              }
+
+              assert LabelsWellDefAux(body', post.scopes.Keys) by {
+                assert desugaredLoop(body')[3] == body';
+                LabelsWellDefSeqToCmd(desugaredLoop(body'), post.scopes.Keys);
+              }
+              EliminateLoopsCorrect(a, body, s', post');
+            }
+
+            calc {
+                WpCmd(a, Loop(invs, body), post)(s);
+                WpCmd(a, SeqToCmd(desugaredLoop(body)), post)(s);
+                { WpSeqToCmdSingleDiff(a, desugaredLoop(body), desugaredLoop(body'), 3, post, s); }
+                WpCmd(a, SeqToCmd(desugaredLoop(body')), post)(s);
+            }
+        case _ => //trivial (EliminateLoops is the identity function here)
+    }
 }
