transformations/Passification.dfy
@@ -4,8 +4,10 @@ include "../dafny-libraries/src/Collections/Maps/Maps.dfy"
 include "../dafny-libraries/src/Math.dfy"
 include "../util/Naming.dfy"
 include "../util/AstSubsetPredicates.dfy"
+include "../util/SortUtil.dfy"
 
-module SSA 
+
+module Passification
 {
 
   import opened BoogieLang
@@ -15,6 +17,7 @@ module SSA
   import opened Naming
   import Maps
   import opened AstSubsetPredicates
+  import SortUtil
 
   type Incarnation<T> = map<var_name, T> 
 
@@ -87,28 +90,31 @@ module SSA
       IncarnationResult_(inputIncMap, globalIncMap', updatedInc)
   }
 
-  function method OutputIncarnation(globalIncMap: Incarnation<nat>, input: Incarnation<var_name>, b: BasicBlock) : (map<var_name, nat>, Incarnation<var_name>, BasicBlock)
+  //TODO: figure out why compiler complains if directly use triple as result type
+  datatype OutputIncRes = OutputIncRes(map<var_name, nat>, Incarnation<var_name>, BasicBlock)
+
+  function method OutputIncarnation(globalIncMap: Incarnation<nat>, input: Incarnation<var_name>, b: BasicBlock) : OutputIncRes
   requires input.Keys <= globalIncMap.Keys
   ensures
-    var (globalIncMap', outputInc, b') := OutputIncarnation(globalIncMap, input, b);
+    var OutputIncRes(globalIncMap', outputInc, b') := OutputIncarnation(globalIncMap, input, b);
     && outputInc.Keys <= globalIncMap'.Keys
     && globalIncMap.Keys <= globalIncMap'.Keys
   decreases b
   {
     match b
-    case Skip => (globalIncMap, input, b)
+    case Skip => OutputIncRes(globalIncMap, input, b)
     case Assert(e) => 
       var e' := e.MultiSubstExpr(input); 
-      (globalIncMap, input, Assert(e'))
+      OutputIncRes(globalIncMap, input, Assert(e'))
     case Assume(e) => 
       var e' := e.MultiSubstExpr(input); 
-      (globalIncMap, input, Assume(e'))
+      OutputIncRes(globalIncMap, input, Assume(e'))
     case Assign(x, t, e) => 
       var e' := e.MultiSubstExpr(input); 
       var counter := if x in globalIncMap.Keys then globalIncMap[x]+1 else 1;
       var x' := VersionedName(x, counter);
 
-      (globalIncMap[x := counter], input[x := x'], Assign(x', t, e'))
+      OutputIncRes(globalIncMap[x := counter], input[x := x'], Assign(x', t, e'))
 
     case Havoc(varDecls) => 
       var delta := map x | x in GetVarNames(varDecls) :: if x in globalIncMap.Keys then globalIncMap[x]+1 else 1;
@@ -119,10 +125,11 @@ module SSA
 
       var varDecls' := Sequences.Map( (vd : VarDecl) requires vd.0 in delta.Keys => (VersionedName(vd.0, delta[vd.0]), vd.1), varDecls);
       
-      (globalIncMap', output, Havoc(varDecls'))
+      OutputIncRes(globalIncMap', output, Havoc(varDecls'))
     case SeqSimple(sc1, sc2) => 
-      var (globalIncMap1, inc1, b1) := OutputIncarnation(globalIncMap, input, sc1);
-      OutputIncarnation(globalIncMap1, inc1, sc2)
+      var OutputIncRes(globalIncMap1, inc1, sc1') := OutputIncarnation(globalIncMap, input, sc1);
+      var OutputIncRes(globalIncMap2, inc2, sc2') := OutputIncarnation(globalIncMap1, inc1, sc2);
+      OutputIncRes(globalIncMap2, inc2, SeqSimple(sc1',sc2'))
   }
 
   datatype SSAResult = 
@@ -158,7 +165,7 @@ module SSA
     if |conflictInc.Keys| == 0 then
       blocks
     else
-      var conflictVarsSeq := Util.SetToSequenceStr(conflictInc.Keys);
+      var conflictVarsSeq := SortUtil.SetToSequenceStr(conflictInc.Keys);
 
       var update := map predId | predId in predIds :: 
         SeqSimple(blocks[predId], SynchronizationBlocks(incs[predId], conflictInc, conflictVarsSeq));
@@ -173,6 +180,10 @@ module SSA
     requires forall id | id in pred.Keys :: forall p | p in pred[id] :: p in cfg.blocks.Keys 
     requires forall block | block in prevResult.incMaps.Keys :: prevResult.incMaps[block].Keys <= prevResult.globalIncMap.Keys
     requires prevResult.incMaps.Keys == set i | 0 <= i < idTopo :: topo[i]
+    requires prevResult.blocks.Keys == set i | 0 <= i < idTopo :: topo[i]
+    ensures   
+      var res := SSAAux(cfg, idTopo, topo, pred, prevResult);
+      res.blocks.Keys == set i | i in topo
     decreases |topo|-idTopo
   {
     if idTopo == |topo| then 
@@ -186,12 +197,12 @@ module SSA
       var incRes := InputIncarnation(prevResult.globalIncMap, predIncs);
 
       /* for each conflict add synchronization assignments */
-      var blocks' := if curId in pred.Keys then AddSynchronizationBlocks(cfg.blocks, prevResult.incMaps, preds, incRes.updatedInc) else cfg.blocks;
+      var blocks' := if curId in pred.Keys then AddSynchronizationBlocks(prevResult.blocks, prevResult.incMaps, preds, incRes.updatedInc) else prevResult.blocks;
       
       /* compute output incarnation of block */
-      var (globalIncMap'', outputIncarnation, b') := OutputIncarnation(incRes.globalIncMap, incRes.localIncMap, cfg.blocks[curId]);
+      var OutputIncRes(globalIncMap'', outputIncarnation, b') := OutputIncarnation(incRes.globalIncMap, incRes.localIncMap, cfg.blocks[curId]);
 
-      var ssaResult' := SSAResult_(prevResult.blocks[curId := b'], prevResult.incMaps[curId := outputIncarnation], globalIncMap'');
+      var ssaResult' := SSAResult_(blocks'[curId := b'], prevResult.incMaps[curId := outputIncarnation], globalIncMap'');
       assert ssaResult'.incMaps.Keys == prevResult.incMaps.Keys + {topo[idTopo]};
       assert (set i | 0 <= i < idTopo :: topo[i]) + {topo[idTopo]} == (set i | 0 <= i < idTopo+1 :: topo[i]);
 
@@ -212,7 +223,9 @@ module SSA
           (forall i | 0 <= i < |pred[blockId]| :: pred[blockId][i] in g.blocks.Keys))
 
       && (forall id | id in pred.Keys :: forall p | p in pred[id] :: p in g.blocks.Keys )
-    
+    ensures 
+      var g' := SSA(g, topo, pred);
+      g'.blocks.Keys == set i | i in topo
   {
     var ssaResult := SSAAux(g, 0, topo, pred, SSAResult_(map[], map[], map[]));
 
@@ -220,6 +233,7 @@ module SSA
   }
 
   function method PassifySimpleCmd(sc: SimpleCmd) : SimpleCmd
+  ensures IsPassive(PassifySimpleCmd(sc))
   {
     match sc
     case Skip => sc
@@ -243,8 +257,9 @@ module SSA
       && (forall blockId | blockId in pred.Keys ::
           (forall i | 0 <= i < |pred[blockId]| :: pred[blockId][i] in g.blocks.Keys))
     ensures 
-      var g := PassifyCfg(g, topo, pred);
-      forall blockId | blockId in g.blocks :: IsPassive(g.blocks[blockId])
+      var g' := PassifyCfg(g, topo, pred);
+      && (forall blockId | blockId in g'.blocks :: IsPassive(g'.blocks[blockId]))
+      && g'.blocks.Keys == set i | i in topo
   {
     var cfgSSA := SSA(g, topo, pred);
     var blocks' := map blockId | blockId in cfgSSA.blocks.Keys :: PassifySimpleCmd(cfgSSA.blocks[blockId]);
