util/CfgHelper.dfy
@@ -1,24 +1,29 @@
 include "../lang/Cfg.dfy"
 include "../dafny-libraries/src/Collections/Sequences/Seq.dfy"
+include "Util.dfy"
 
 module CfgHelper {
   import opened BoogieCfg
   import Sequences = Seq
+  import Util
 
   type Graph<T> = map<T, seq<T>>
 
   /** Topological order */
 
-  /** would like to use Sequences.FoldLeft instead of a separate method here,
-  but not sure how to get the termination constraints right */
   function method TopologicalOrderAuxSeq<T>(
     succ: Graph<T>, 
     ns: seq<T>, 
     visitedAndStack: (set<T>, seq<T>)
     ) : (set<T>, seq<T>)
+    requires GraphWf(succ)
+    requires (forall n | n in ns :: n in succ.Keys)
+    requires (forall n | n in visitedAndStack.1 :: n in succ.Keys)
     decreases succ.Keys - visitedAndStack.0, 1, ns
     ensures
       var res := TopologicalOrderAuxSeq(succ, ns, visitedAndStack);
+
+      && (forall n | n in res.1 :: n in succ.Keys)
       && visitedAndStack.0 <= res.0      
       //&& (forall n | n in ns :: n !in visitedAndStack.0 ==> n in res.1)
   {
@@ -33,12 +38,18 @@ module CfgHelper {
     n: T, 
     visitedAndStack: (set<T>, seq<T>)
     ) : (set<T>, seq<T>)
+    requires GraphWf(succ)
+    requires n in succ.Keys
+    requires (forall n | n in visitedAndStack.1 :: n in succ.Keys)
     ensures
       var (visited', stack'):= TopologicalOrderAux(succ, n, visitedAndStack);
+      && (forall n | n in stack' :: n in succ.Keys)
       && visitedAndStack.0 <= visited'      
       && ((n !in visitedAndStack.0) ==> 
               && n in visited'
-              && stack'[0] == n)
+              && stack'[0] == n) 
+      //&& Sequences.HasNoDuplicates(stack')
+      //&& visitedStack.1 <= 
     decreases succ.Keys - visitedAndStack.0, 0
   {
     var (visited, stack) := visitedAndStack;
@@ -47,6 +58,7 @@ module CfgHelper {
     else 
       var visited' := visited + {n};
       var successors : seq<T> := if n in succ.Keys then succ[n] else [];
+      assert n in succ.Keys;
       var (visitedRes, stackRes) :=
         if n in succ.Keys then
           TopologicalOrderAuxSeq(succ, succ[n], (visited', stack))
@@ -56,11 +68,75 @@ module CfgHelper {
       (visitedRes, [n]+stackRes)
   }
 
-  function method TopologicalOrder(cfg: Cfg, blocksSeq: seq<BlockId>) : seq<BlockId>
+  function method TopologicalOrder(cfg: Cfg) : seq<BlockId>
+    requires CfgWf(cfg)
+    //&& forall n | n in blocksSeq :: n in cfg.successors.Keys
+    ensures
+      var res := TopologicalOrder(cfg);
+      (forall n | n in res :: n in cfg.successors.Keys)
   {
-    TopologicalOrderAuxSeq(cfg.successors, blocksSeq, ({}, [])).1
+    //TopologicalOrderAuxSeq(cfg.successors, blocksSeq, ({}, [])).1
+    TopologicalOrderAux(cfg.successors, cfg.entry, ({}, [])).1
   }
 
+  /*
+  lemma TopologicalOrderAuxSeqCorrect(
+    succ: Graph<BlockId>, 
+    ns: seq<BlockId>, 
+    visitedAndStack: (set<BlockId>, seq<BlockId>),
+    cover: set<BlockId>
+  )
+    requires IsAcyclicSeq(succ, ns, cover)
+    requires GraphWf(succ)
+    requires n in succ.Keys
+    requires (forall n | n in visitedAndStack.1 :: n in succ.Keys)
+    ensures
+      var (visited', stack'):= TopologicalOrderAux(succ, n, visitedAndStack);
+      forall i | 0 <= i < |stack'| :: (set nSucc | nSucc in succ[stack'[i]]) <=  (set j | 0 < j < |stack'| :: stack'[j]) 
+    */
+
+  /*
+  lemma TopologicalOrderAuxCorrect(
+    succ: Graph<BlockId>, 
+    n: BlockId, 
+    visitedAndStack: (set<BlockId>, seq<BlockId>),
+    cover: set<BlockId>
+  )
+    requires IsAcyclic(succ, n, cover)
+    requires GraphWf(succ)
+    requires n in succ.Keys
+    requires (forall n | n in visitedAndStack.1 :: n in succ.Keys)
+    ensures
+      var (visited', stack'):= TopologicalOrderAux(succ, n, visitedAndStack);
+      //forall i | 0 <= i < |stack'| :: (set nSucc | nSucc in succ[stack'[i]]) <=  (set j | i < j < |stack'| :: stack'[j]) 
+      forall i | 0 <= i < |stack'| :: test(succ[stack'[i]]) <=  test(stack'[i+1..|stack'|])
+
+  function test<T>(xs: seq<T>) : set<T>
+  {
+    set x | x in xs
+  }
+
+  lemma TopologicalOrderCorrect(
+    cfg: Cfg, 
+    cover: set<BlockId>
+  )
+    requires CfgWf(cfg)
+    requires
+      var succ := cfg.successors;
+      && IsAcyclic(succ, cfg.entry, cover)
+      && GraphWf(succ)
+      && cfg.entry in succ.Keys
+    ensures
+      var succ := cfg.successors;
+      var topo := TopologicalOrder(cfg);
+      forall i 
+        | 0 <= i < |topo| 
+        :: test(succ[topo[i]]) <=  test(topo[i+1..|topo|]) 
+  {
+    var (_, topo):= TopologicalOrderAux(cfg.successors, cfg.entry, ({}, []));
+    TopologicalOrderAuxCorrect(cfg.successors, cfg.entry, ({}, []), cover);
+  }
+  */
   
   /** Predecessor map */
   function method PredecessorMap<T>(succ: Graph<T>, ns: seq<T>) : Graph<T>
@@ -75,10 +151,12 @@ module CfgHelper {
   }
 
   lemma PredecessorMapCorrect<T>(succ: Graph<T>, ns: seq<T>)
-  requires succ.Keys <= set n | n in ns :: n
-  ensures
-    var pred := PredecessorMap(succ, ns);
+    requires succ.Keys <= set n | n in ns :: n
+    requires GraphWf(succ)
+    ensures
+      var pred := PredecessorMap(succ, ns);
 
+    && pred.Keys <= succ.Keys
     /** only predecessors are recorded  */
     && (forall n | n in pred.Keys :: forall p | p in pred[n] :: p in succ.Keys && n in succ[p])
     /** every predecessor is recorded */
@@ -99,6 +177,85 @@ module CfgHelper {
     var inv2 := (pred: Graph<T>, ns: seq<T>) => 
       (forall n | n in succ.Keys && n !in ns :: forall s | s in succ[n] :: s in pred.Keys && n in pred[s]);
     Sequences.LemmaInvFoldLeft(inv2, stp, f, map [], ns);
+
+
+    var inv3 := (pred: Graph<T>, ns: seq<T>) => pred.Keys <= succ.Keys;
+    Sequences.LemmaInvFoldLeft(inv3, stp, f, map [], ns);
+  }
+
+  lemma ConvertTopo(succ: map<BlockId, seq<BlockId>>, pred: map<BlockId, seq<BlockId>>, topo: seq<BlockId>)
+    requires forall n | n in topo :: n in succ.Keys
+    requires forall n | n in succ.Keys :: n in topo
+    requires forall i | 0 <= i < |topo| :: (set nSucc | nSucc in succ[topo[i]]) <=  (set j | i < j < |topo| :: topo[j]) 
+    requires Sequences.HasNoDuplicates(topo)
+    requires
+      && pred.Keys <= succ.Keys
+      /** only predecessors are recorded  */
+      && (forall n | n in pred.Keys :: forall p | p in pred[n] :: p in succ.Keys && n in succ[p])
+      /** every predecessor is recorded */
+      && (forall n | n in succ.Keys :: forall s | s in succ[n] :: s in pred.Keys && n in pred[s])
+    ensures forall i | 0 <= i < |topo| :: topo[i] in pred.Keys ==> (set x | x in pred[topo[i]]) <= (set j | 0 <= j < i :: topo[j])
+  {
+    forall i | 0 <= i < |topo| && topo[i] in pred.Keys
+    ensures (set x | x in pred[topo[i]]) <= (set j | 0 <= j < i :: topo[j])
+    {
+      forall x | x in pred[topo[i]]
+      ensures x in (set j | 0 <= j < i :: topo[j])
+      {
+
+        if x !in (set j | 0 <= j < i :: topo[j]) {
+          var xIdx :| i <= xIdx < |topo| && topo[xIdx] == x;
+          assert topo[i] in succ[topo[xIdx]];
+
+          var xs := (set nSucc | nSucc in succ[topo[xIdx]]);
+          var ys := (set j | xIdx < j < |topo| :: topo[j]);
+
+          assert xs <= ys;
+          assert topo[i] in xs;
+          assert topo[i] in ys;
+
+          assert false by {
+            var k :| xIdx < k < |topo| && topo[i] == topo[k];
+            reveal Sequences.HasNoDuplicates();
+          }
+        }
+      }
+    }
+  }
+
+  function method PrintCfgAux(cfg: Cfg, blockIds: seq<BlockId>, idx: BlockId) : string
+    requires CfgWf(cfg)
+    requires forall id | id in blockIds :: id in cfg.blocks.Keys && id in cfg.successors.Keys
+    decreases |blockIds|-idx
+  {
+    if idx >= |blockIds| then
+      ""
+    else
+      var bId := blockIds[idx];
+      var blockName := "B"+Util.NatToString(bId);
+      var blockString := cfg.blocks[bId].ToString(0);
+      var successors := cfg.successors[bId];
+
+      "\n"+blockName+":\n"+
+      blockString+"\n"+
+      (
+      if successors == [] then 
+        "return;\n"
+      else
+        Sequences.FoldLeft( 
+            (s: string, bSucc: BlockId) => 
+              if bSucc in cfg.blocks.Keys then s+", B"+ Util.NatToString(bSucc) else "block not in successors",
+            "targets: ",
+            successors)+"\n"
+      ) +
+      PrintCfgAux(cfg, blockIds, idx+1)
+  }
+
+  function method PrintCfg(cfg: Cfg, blockIds: seq<BlockId>) : string
+    requires CfgWf(cfg)
+    requires forall id | id in blockIds :: id in cfg.blocks.Keys
+  {
+    PrintCfgAux(cfg, blockIds, 0)
   }
 
 }
