util/Util.dfy
@@ -2,16 +2,15 @@ include "../dafny-libraries/src/Wrappers.dfy"
 include "../dafny-libraries/src/Collections/Sequences/Seq.dfy"
 
 module Util {
-
   import opened Wrappers
   import Seq
 
-  function RemoveDuplicates<T>(s: seq<T>): seq<T>
+  function method RemoveDuplicates<T(==)>(s: seq<T>): seq<T>
   {
     RemoveDuplicatesAux(s, {})
   }
 
-  function RemoveDuplicatesAux<T>(s: seq<T>, alreadyIncluded: set<T>): seq<T>
+  function method RemoveDuplicatesAux<T>(s: seq<T>, alreadyIncluded: set<T>): seq<T>
   {
     if |s| == 0 then []
     else 
@@ -21,29 +20,7 @@ module Util {
         [s[0]] + RemoveDuplicatesAux(s[1..], {s[0]}+alreadyIncluded)
   }
 
-  method IntToString(i: int) returns (s: string) {
-    if i == 0 {
-      return "0";
-    } 
-
-    s := "";
-    var j := i;
-
-    if i < 0 {
-      s := "-";
-      j := -i;
-    }
-
-    while j != 0
-      invariant j >= 0;
-    {
-      var d := j % 10;
-      s := ['0' + d as char] + s;
-      j := j / 10;
-    }
-  }
-
-  function method IntToString2(i: int) : string {
+  function method IntToString(i: int) : string {
     if i < 0 then "-"+NatToString(-i) else NatToString(i)
   }
 
@@ -52,7 +29,8 @@ module Util {
     else 
       var digit := n % 10;
       var digitString := ['0' + digit as char];
-      digitString + NatToString(n/10)
+      var remainder := n/10;
+      (if remainder > 0 then NatToString(n/10) else "") + digitString
   }
 
   lemma HashTagNotInNatString(n: nat)
@@ -62,32 +40,41 @@ module Util {
   lemma NatToStringInjective(n1: nat, n2: nat)
     requires n1 != n2
     ensures NatToString(n1) != NatToString(n2)
-  /*
   {
     if n1 == 0 {
-      //trivial
+      assert n2 != 0;
+      var digit2 := n2 % 10;
+
+      var digitString2 := ['0' + digit2 as char];
+      var remainder2 := n2/10;
+
+      assert "0"[0] == '0'+ 0 as char;
     } else {
       var digit1 := n1 % 10;
       var digitString1 := ['0' + digit1 as char];
+      var remainder1 := n1/10;
+      var res1 := (if remainder1 > 0 then NatToString(n1/10) else "") + digitString1;
 
       var digit2 := n2 % 10;
       var digitString2 := ['0' + digit2 as char];
+      var remainder2 := n2/10;
+      var res2 := (if remainder2 > 0 then NatToString(n2/10) else "")+ digitString2;
 
       assert |digitString1| == |digitString2|;
 
-      assume NatToString(n1/10) != NatToString(n2/10);
-
       if digit1 != digit2 {
-        //assert ('0'+ digit1 as char) != ('1'+ digit2 as char);
-        assume false;
+        assert ('0'+ digit1 as char) != ('0'+ digit2 as char);
+        assert digitString1 != digitString2;
+        assert res1[|res1|-1] != res2[|res2|-1];
       } else {
-        assume n1/10 != n2/10;
-        NatToStringInjective(n1/10, n2/10);
-
+        assert NatToString(n1/10) != NatToString(n2/10) by {
+          assert n1/10 != n2/10;
+          NatToStringInjective(n1/10, n2/10);
+        }
+        assert res1[0..|res1|-1] != res2[0..|res2|-1];
       }
     }
   }
-  */
 
   function method BoolToString(b: bool) : string {
     if b then "true" else "false"
@@ -116,326 +103,4 @@ module Util {
     case Some(true) =>
     case Some(false) =>
   }
-
-  predicate method LexRelStr(s1: string, s2: string)
-  {
-    || s1 == []
-    || (s2 != [] && s1[0] < s2[0]) 
-    || (s2 != [] && s1[0] == s2[0] && LexRelStr(s1[1..], s2[1..]))
-  }
-
-  lemma LexRelConnex(s1: string, s2: string)
-    ensures LexRelStr(s1, s2) || LexRelStr(s2, s1)
-  { }
-
-  lemma LexRelAntisym(s1: string, s2: string)
-    requires LexRelStr(s1, s2)
-    requires LexRelStr(s2, s1)
-    ensures s1 == s2
-  { }
-
-  lemma LexRelTransitive(s1: string, s2: string, s3: string)
-    requires LexRelStr(s1, s2)
-    requires LexRelStr(s2, s3)
-    ensures LexRelStr(s1, s3)
-  { }
-
-  lemma LexRelIsTotalOrder()
-  ensures IsTotalOrder(LexRelStr)
-  {
-    forall s1, s2
-    ensures LexRelStr(s1, s2) || LexRelStr(s2, s1)
-    { LexRelConnex(s1, s2); }
-
-    forall s1, s2 | LexRelStr(s1, s2) && LexRelStr(s2, s1)
-    ensures s1 == s2
-    { LexRelAntisym(s1, s2); }
-
-    forall s1, s2, s3 | LexRelStr(s1, s2) && LexRelStr(s2, s3)
-    ensures LexRelStr(s1, s3)
-    { LexRelTransitive(s1, s2, s3); }
-  }
-
-  /** 
-  Various of the following definitions and lemmas are taken from http://leino.science/papers/krml275.html
-  */
-
-  predicate IsTotalOrder<A(!new)>(R: (A, A) -> bool) {
-    // connexity
-    && (forall a, b :: R(a, b) || R(b, a))
-    // antisymmetry
-    && (forall a, b :: R(a, b) && R(b, a) ==> a == b)
-    // transitivity
-    && (forall a, b, c :: R(a, b) && R(b, c) ==> R(a, c))
-  }
-
-  lemma ThereIsAMinimumGeneral<A>(R: (A, A) -> bool, s: set<A>)
-    requires s != {}
-    requires IsTotalOrder(R)
-    ensures exists x :: x in s && forall y | y in s :: R(x, y)
-  {
-    var x :| x in s;
-    if s == {x} {
-      // obviously, x is the minimum
-      assert x in s;
-      assert forall y | y in s :: x == y;
-    } else {
-      // The minimum in s might be x, or it might be the minimum
-      // in s - {x}. If we knew the minimum of the latter, then
-      // we could compare the two.
-      // Let's start by giving a name to the smaller set:
-      var s' := s - {x};
-      // So, s is the union of s' and {x}:
-      assert s == s' + {x};
-      // The following lemma call establishes that there is a
-      // minimum in s'.
-      ThereIsAMinimumGeneral(R, s');
-      var x' :| x' in s' && forall y | y in s' :: R(x', y);
-
-      var xMin := if R(x, x') then x else x';
-
-      assert xMin in s;
-
-      forall y | y in s
-      ensures R(xMin, y)
-      {
-      }
-    }
-  }
-
-  lemma ThereIsAMinimum(s: set<string>)
-    requires s != {}
-    ensures exists x :: x in s && forall y | y in s :: LexRelStr(x, y)
-  {
-    assert IsTotalOrder(LexRelStr) by {
-      LexRelIsTotalOrder();
-    }
-
-    ThereIsAMinimumGeneral(LexRelStr, s);
-  }  
-
-  predicate Sorted(a: array<string>, low: int, high: int)
-    requires 0 <= low <= high <= a.Length
-    reads a
-  {
-    forall i, j :: low <= i < j < high ==> LexRelStr(a[i], a[j])
-  }
-
-  predicate SortedSeq(a: seq<string>, low: int, high: int)
-    requires 0 <= low <= high <= |a|
-  {
-    forall i, j :: low <= i < j < high ==> LexRelStr(a[i], a[j])
-  }
-
-  lemma UniqueMinimum(x1: string, x2: string, s: set<string>)
-  requires x1 in s && x2 in s
-  requires forall x | x in s :: LexRelStr(x1,x)
-  requires forall x | x in s :: LexRelStr(x2,x)
-  ensures x1 == x2
-  {
-    assert LexRelStr(x1, x2) || LexRelStr(x2, x1) by {
-      LexRelConnex(x1, x2);
-    }
-
-    if LexRelStr(x1, x2) && LexRelStr(x2, x1) {
-      assert x1 == x2 by {
-        LexRelAntisym(x1, x2);
-      }
-    }
-  }
-
-  lemma CardMono<A>(s1: set<A>, s2: set<A>)
-  requires s1 <= s2
-  ensures |s1| <= |s2|
-  {
-    if s1 == {} {
-
-    } else {
-      var x :| x in s1;
-      assert x in s2;
-
-      assert |s1-{x}| <= |s2-{x}| by {
-        CardMono(s1-{x}, s2-{x});
-      }
-    }
-  }
-
-  lemma CardSeqSet<A>(s: seq<A>)
-  ensures |s| >= |(set x | x in s)|
-  {
-    if |s| == 0 {
-
-    } else {
-      var xs := set x | x in s;
-      assert s[0] in xs;
-
-      var xs' := xs-{s[0]};
-
-      calc {
-        |s|;
-        |s[1..]|+1;
-      >= { CardSeqSet(s[1..]); }
-        |(set x | x in s[1..])|+1;
-      >=
-        { 
-          assert (set x | x in s[1..]) >= xs';
-          CardMono(xs', set x | x in s[1..]);
-        }
-        |xs'|+1;
-      }
-    }
-  }
-
-  lemma SortedUnique(s1: seq<string>, s2: seq<string>, xs: set<string>)
-    requires |s1| == |s2| == |xs|
-    requires (set x | x in s1) == (set x | x in s2) == xs
-    requires SortedSeq(s1, 0, |s1|)
-    requires SortedSeq(s2, 0, |s2|)
-    ensures s1 == s2
-  {
-    if xs == {} {
-    } else {
-      assert IsTotalOrder(LexRelStr) by {
-        LexRelIsTotalOrder();
-      }
-
-      assert forall y | y in xs :: LexRelStr(s1[0], y);
-      assert forall y | y in xs :: LexRelStr(s2[0], y);
-
-      assert s1[0] == s2[0] by {
-        UniqueMinimum(s1[0], s2[0], xs);
-      }
-
-      assert s1[1..] == s2[1..] by {
-        assert (set x | x in s1[1..]) + {s1[0]} == xs;
-        assert |s1[1..]| == |xs|-1;
-
-        if s1[0] in (set x | x in s1[1..]) {
-          assert (set x | x in s1[1..]) == xs;
-          assert |s1[1..]| >= |xs| by {
-            CardSeqSet(s1[1..]);
-          }
-          assert false;
-        }
-
-        if s2[0] in (set x | x in s2[1..]) {
-          assert (set x | x in s2[1..]) == xs;
-          assert |s2[1..]| >= |xs| by {
-            CardSeqSet(s2[1..]);
-          }
-          assert false;
-        }
-
-        SortedUnique(s1[1..], s2[1..], xs-{s1[0]});
-      }
-    }
-  }
-
-  method Sort(a: array<string>)
-    modifies a
-    ensures 
-      && Sorted(a, 0, a.Length)
-      && multiset(a[..]) == old(multiset(a[..]))
-    
-  lemma MultisetEmpty<A>(s: seq<A>)
-  requires multiset(s) == multiset{};
-  ensures s == []
-  {
-    if s != [] {
-      assert s[0] in multiset(s);
-      assert false;
-    } 
-  }
-
-  lemma MultisetNonempty<A>(s: seq<A>)
-  requires s != []
-  ensures multiset(s) != multiset{}
-  {
-    assert s[0] in multiset(s);
-  }
-  
-  lemma MultisetToSetSeq<A>(s1: seq<A>, s2: seq<A>)
-  requires multiset(s1) == multiset(s2)
-  ensures (set i | i in s1) == (set i | i in s2)
-  {
-    var s1Set := (set i | i in s1);
-    var s2Set := (set i | i in s2);
-
-    forall x | x in s1Set
-    ensures x in s2Set
-    {
-      assert x in multiset(s1);
-    }
-
-    forall x | x in s2Set
-    ensures x in s1Set
-    {
-      assert x in multiset(s2);
-    }
-  }
-
-  function SetToSequenceStr(s: set<string>) : seq<string>
-    ensures 
-      var res := SetToSequenceStr(s);
-      && (set x | x in res) == s
-      && |s| == |res|
-      && SortedSeq(res, 0, |res|)
-  {
-    if s == {} then
-      []
-    else
-      ThereIsAMinimum(s);
-      var min :| min in s && forall s' | s' in s :: LexRelStr(min, s');
-
-      assert {min}+(s-{min}) == s;
-
-      [min] + SetToSequenceStr(s-{min})
-  } by method {
-    var a: array<string> := new string[|s|];
-
-    var i := 0;
-    var s' := s;
-    while i < |s|
-      decreases s'
-      invariant |s'| == |s|-i
-      invariant 0 <= i <= |s|
-      invariant (set j | j in a[0..i]) == s-s'
-    {
-      var x :| x in s';
-
-      var a0Seq := a[..];
-
-      a[i] := x;
-
-      assert forall j | 0 <= j < i :: a[j] == a0Seq[j];
-      assert (set j | j in a[0..i]) == s-s';
-
-      var temp := s';
-      s' := s' - {x};
-
-      assert (set j | j in a[0..i+1]) == (s-temp)+{x};
-      i := i+1;
-    }
-
-    assert i == |s|;
-
-    assert (set j | j in a[0..i]) == s;
-    assert (set j | j in a[..]) == s;
-    var a0 := a[..];
-    
-    Sort(a);
-    
-    MultisetToSetSeq(a[..], a0);
-    
-    assert (set j | j in a[..]) == s;
-
-    var res := a[..];
-
-    assert res == SetToSequenceStr(s) by {
-      SortedUnique(res, SetToSequenceStr(s), s);
-    }
-
-    return res;
-  }
-
 }
