transformations/AllTransformations.dfy
@@ -1,0 +1,198 @@
+/** Top-level module that invokes all the Boogie transformations */
+
+include "LoopElim.dfy"
+include "IfGuardElim.dfy"
+include "DesugarScopedVarsImpl.dfy"
+include "NormalizeAst.dfy"
+include "AstToCfg_simple.dfy"
+include "Passification.dfy"
+include "VCGen.dfy"
+include "../lang/BoogieLang.dfy"
+include "../lang/Cfg.dfy"
+include "../util/AstSubsetPredicates.dfy"
+include "../util/CfgHelper.dfy"
+include "../smt_interface/SMTInterface.dfy"
+
+module AllTransformations
+{
+
+  import opened BoogieLang 
+  import opened Wrappers
+  import opened AstSubsetPredicates
+
+  import LoopElim
+  import IfGuardElim
+  import DesugarScopedVarsImpl
+  import NormalizeAst
+  import AstToCfg
+  import Passification
+  import VCGen
+  import CfgHelper
+  import BoogieCfg
+
+  method AllTransformations(c: Cmd) returns (e: Expr)
+    requires NoBreaks(c) //TODO: lift
+  {
+    /** Eliminate loops */
+    var c1 := LoopElim.EliminateLoops(c); 
+
+    LoopElim.EliminateLoopsPreserveNoBreaks(c);
+
+    print("\n=====After loop elimination=====\n");
+    print(c1.ToString(0));
+
+    /** Eliminate if guards */
+    var c2 := IfGuardElim.EliminateIfGuards(c1); 
+    print("\n=====After If guard elimination=====\n");
+    print(c2.ToString(0));
+
+    IfGuardElim.EliminateIfGuardsNoLoops(c1);
+
+    /** Remove scoped variables */
+    var (c3, decls3) := DesugarScopedVarsImpl.RemoveScopedVars(c2);
+    DesugarScopedVarsImpl.RemoveScopedVarsStructure(c2);
+    print("\n=====After removing scoped variables=====\n");
+    print(c3.ToString(0));
+
+    /** Normalize AST */
+    var (c4Opt, scExitOpt) := NormalizeAst.NormalizeAst(c3, None);
+    var c4 := NormalizeAst.SeqCmdSimpleOpt(c4Opt, scExitOpt);
+    print("\n=====After AST normalization=====\n");
+    print(c4.ToString(0));
+
+    NormalizeAst.NormalizeAstPreserveStructure(c3, None);
+
+    assert NoBreaks(c4);
+    assert NoLoopsNoIfGuardNoScopedVars(c4) && NoBreaks(c4);
+    
+    /** Ast-to-CFG */
+    var (g1, blockSeq, cover) := AstToCfg.AstToCfg(c4);
+    print("\n=====After AST-to-CFG transformation=====\n");
+    print(CfgHelper.PrintCfg(g1, blockSeq));
+
+    /** Compute auxiliary CFG data */
+    var pred := CfgHelper.PredecessorMap(g1.successors, blockSeq);
+
+    CfgHelper.PredecessorMapCorrect(g1.successors, blockSeq);
+
+    var topo := CfgHelper.TopologicalOrder(g1);
+
+    //CfgHelper.TopologicalOrderCorrect(g1, cover);
+    
+    expect (forall i | 0 <= i < |topo| :: topo[i] in pred.Keys ==> 
+    (set x | x in pred[topo[i]]) <= (set j | 0 <= j < i :: topo[j]));
+
+    /** Passification */
+    var g2 := Passification.PassifyCfg(g1, topo, pred);
+    print("\n=====After Passification=====\n");
+    expect BoogieCfg.CfgWf(g2);
+
+    print(CfgHelper.PrintCfg(g2, topo));
+
+    /** VCGen */
+    expect g2.entry == topo[0];
+
+    var vc := 
+      if |topo| == 0 then
+        Expr.TrueExpr
+      else 
+        VCGen.GenerateVC(g2, topo);
+
+    return vc;
+  }
+  
+}
+
+import opened BoogieLang
+import opened Wrappers
+import opened SMTInterface
+
+module Environment {
+  method {:extern "Shims", "GetCommandLineArguments"} GetCommandLineArguments() returns (args: seq<string>)
+}
+
+method Main()
+{
+  /*
+  var c := 
+    Scope(
+      None,
+      [("x", TPrim(TInt))], 
+      Seq(
+        SimpleCmd(Assume(BinOp(Var("x"), Gt, ELit(LitInt(0))))),
+        SimpleCmd(Assert(BinOp(Var("x"), Gt, ELit(LitInt(1)))))
+      )
+    );
+  */
+  /*
+  var c :=
+    Scope(
+      None,
+      [("x", TPrim(TInt)), ("y", TPrim(TInt))], 
+      If(Some(BinOp(Var("x"), Gt, ELit(LitInt(0)))),
+        SimpleCmd(Assert(BinOp(Var("x"), Gt, ELit(LitInt(0))))),
+        SimpleCmd(Assert(BinOp(Var("x"), Le, ELit(LitInt(0)))))
+      )
+    );
+  */
+  /*
+  var c :=
+    Scope(
+      None,
+      [("x", TPrim(TInt)), ("y", TPrim(TInt))], 
+      Seq(
+        SimpleCmd(Assign("x", TPrim(TInt), ELit(LitInt(0)))),
+        Seq(
+          SimpleCmd(Assign("x", TPrim(TInt), BinOp(Var("x"), Add, ELit(LitInt(1))))),
+          SimpleCmd(Assert(BinOp(Var("x"), Gt, ELit(LitInt(0)))))
+        )
+      )
+    );
+  */
+
+  var c :=
+    Scope(
+      None,
+      [("x", TPrim(TInt)), ("y", TPrim(TInt))], 
+      Seq(
+        Seq(
+          SimpleCmd(Assign("x", TPrim(TInt), ELit(LitInt(1234)))),
+          If(Some(BinOp(Var("x"), Gt, ELit(LitInt(0)))),
+            SimpleCmd(Assign("x", TPrim(TInt), BinOp(Var("x"), Add, ELit(LitInt(1))))),
+            SimpleCmd(Assign("x", TPrim(TInt), BinOp(Var("x"), Add, ELit(LitInt(2)))))
+          )
+        ),
+        SimpleCmd(Assert(BinOp(Var("x"), Gt, ELit(LitInt(0)))))
+      )
+    );
+  
+  var args := Environment.GetCommandLineArguments();
+  if |args| != 2 {
+    print "Expecting exactly two arguments [prover_path] [prover_log_output]";
+    return;
+  }
+
+  var proverPath := args[0];
+  var proverLogPath := args[1];
+  
+  var vc := AllTransformations.AllTransformations(c);
+  var vcString := vc.ToString();
+
+  print("\n=====VC Generation====\n");
+
+  print(vcString+"\n");
+
+  print("\n=====Result=====\n");
+
+  var vcExprInterface := VCExprInterface.Create(proverPath, proverLogPath);
+  
+  var vcExpr := VCExprAdapter.ExprToVCExpr(vcExprInterface, vc);
+  var vcValid := vcExprInterface.IsVCValid(vcExpr);
+
+  if vcValid {
+    print("Input program is correct.");
+  } else {
+    print("Input program might not be correct.");
+  }
+
+}
