transformations/IfGuardElim.dfy
@@ -1,0 +1,149 @@
+include "../lang/BoogieLang.dfy"
+include "../lang/BoogieSemantics.dfy"
+include "../dafny-libraries/src/Wrappers.dfy"
+include "../util/AstSubsetPredicates.dfy"
+include "../util/SemanticsUtil.dfy"
+include "../util/Util.dfy"
+
+
+module IfGuardElim {
+  import opened BoogieLang
+  import opened BoogieSemantics
+  import opened Wrappers
+  import opened AstSubsetPredicates
+  import opened SemanticsUtil
+  import Util
+
+  function method EliminateIfGuards(c: Cmd) : Cmd
+    ensures NoIfGuard(EliminateIfGuards(c))
+  {
+    match c
+    case SimpleCmd(sc) => c
+    case Break(_) => c
+    case Scope(optLabel, varDecls, body) =>
+      var body' := EliminateIfGuards(body);
+      Scope(optLabel, varDecls, body')
+    case If(optGuard, thn, els) =>
+      var thn' := EliminateIfGuards(thn);
+      var els' := EliminateIfGuards(els);
+      if optGuard.Some? then
+        var guard := optGuard.value;
+        assert NoIfGuard(Seq(SimpleCmd(Assume(guard)), thn'));
+        assert NoIfGuard(Seq(SimpleCmd(Assume(UnOp(Not, guard))), els'));
+        If(None, Seq(SimpleCmd(Assume(guard)), thn'), Seq(SimpleCmd(Assume(UnOp(Not, guard))), els'))
+      else
+        If(None, thn', els')
+    case Loop(invs, body) =>
+      var body' := EliminateIfGuards(body);
+      Loop(invs, body')
+    case Seq(c1, c2) =>
+      var c1' := EliminateIfGuards(c1);
+      var c2' := EliminateIfGuards(c2);
+      Seq(c1', c2')
+  }
+
+  lemma EliminateIfGuardsNoLoops(c: Cmd)
+    requires NoLoops(c) && NoBreaks(c)
+    ensures NoLoops(EliminateIfGuards(c)) && NoBreaks(EliminateIfGuards(c))
+  { 
+    match c
+    case If(optGuard, thn, els) =>
+      var thn' := EliminateIfGuards(thn);
+      var els' := EliminateIfGuards(els);
+      if optGuard.Some? {
+        var guard := optGuard.value;
+        assert NoLoops(Seq(SimpleCmd(Assume(guard)), thn'));
+        assert NoLoops(Seq(SimpleCmd(Assume(UnOp(Not, guard))), els'));
+        assert NoBreaks(Seq(SimpleCmd(Assume(guard)), thn'));
+        assert NoBreaks(Seq(SimpleCmd(Assume(UnOp(Not, guard))), els'));
+      }
+    case _ => 
+  }
+
+  lemma EliminateIfGuardsCorrect<A(!new)>(a: absval_interp<A>, c: Cmd, s: state<A>, post: WpPost)
+  requires NoLoops(c)
+  requires LabelsWellDefAux(c, post.scopes.Keys) && LabelsWellDefAux(EliminateIfGuards(c), post.scopes.Keys)
+  ensures WpCmd(a, EliminateIfGuards(c), post)(s) == WpCmd(a, c, post)(s)
+  {
+    reveal WpCmd();
+    match c
+    case Seq(c1, c2) => 
+      var c2Post := WpCmd(a, c2, post);
+      var c2ElimPost := WpCmd(a, EliminateIfGuards(c2), post);
+
+      forall s':state<A> | true
+          ensures c2ElimPost(s') == c2Post(s')
+      {
+        EliminateIfGuardsCorrect(a, c2, s', post);
+      }
+
+      calc {
+        WpCmd(a, EliminateIfGuards(c), post)(s);
+        WpCmd(a, c1, WpPost(c2ElimPost, post.currentScope, post.scopes))(s); 
+        { 
+          WpCmdPointwise(a, c1, WpPost(c2ElimPost, post.currentScope, post.scopes), WpPost(c2Post, post.currentScope, post.scopes), s);
+        }
+        WpCmd(a, c1, WpPost(c2Post, post.currentScope, post.scopes))(s);
+      }
+    case If(optGuard, thn, els) =>
+      var thn' := EliminateIfGuards(thn);
+      var els' := EliminateIfGuards(els);
+
+      if optGuard.Some? {
+        var guard := optGuard.value;
+        
+        calc {
+          WpCmd(a, If(Some(guard), thn, els), post)(s); 
+          { WpShallowIfEquiv(a, guard, thn, els, post, s); }
+          WpCmd(a, If(None, Seq(SimpleCmd(Assume(guard)), thn), Seq(SimpleCmd(Assume(UnOp(Not, guard))), els)), post)(s);
+          Util.AndOpt(
+            WpCmd(a, Seq(SimpleCmd(Assume(guard)), thn), post)(s),
+            WpCmd(a, Seq(SimpleCmd(Assume(UnOp(Not, guard))), els), post)(s)
+          );
+          Util.AndOpt(
+            WpCmd(a, SimpleCmd(Assume(guard)), WpPost(WpCmd(a, thn, post), post.currentScope, post.scopes))(s),
+            WpCmd(a, SimpleCmd(Assume(UnOp(Not, guard))), WpPost(WpCmd(a, els, post), post.currentScope, post.scopes))(s)
+          );
+          { 
+            forall s | true
+            ensures WpCmd(a, thn, post)(s) == WpCmd(a, thn', post)(s)
+            {
+              EliminateIfGuardsCorrect(a, thn, s, post);
+            }
+
+            forall s | true
+            ensures WpCmd(a, els, post)(s) == WpCmd(a, els', post)(s)
+            {
+              EliminateIfGuardsCorrect(a, els, s, post);
+            }
+            WpCmdPointwise2(a, SimpleCmd(Assume(guard)), WpPost(WpCmd(a, thn, post), post.currentScope, post.scopes), 
+              WpPost(WpCmd(a, thn', post), post.currentScope, post.scopes));
+            WpCmdPointwise2(a, SimpleCmd(Assume(guard)), WpPost(WpCmd(a, els, post), post.currentScope, post.scopes), 
+              WpPost(WpCmd(a, els', post), post.currentScope, post.scopes));
+          }
+          Util.AndOpt(
+            WpCmd(a, SimpleCmd(Assume(guard)), WpPost(WpCmd(a, thn', post), post.currentScope, post.scopes))(s),
+            WpCmd(a, SimpleCmd(Assume(UnOp(Not, guard))), WpPost(WpCmd(a, els', post), post.currentScope, post.scopes))(s)
+          );
+        }
+      }    
+    case Scope(optLabel, varDecls, body) => 
+      var updatedScopes := if optLabel.Some? then post.scopes[optLabel.value := post.normal] else post.scopes;
+      assert updatedScopes.Keys == if optLabel.Some? then {optLabel.value} + post.scopes.Keys else post.scopes.Keys;
+
+      var bodyPost := ResetVarsPost(varDecls, WpPost(post.normal, post.normal, updatedScopes), s);
+
+      forall s: state<A> | true 
+        ensures WpCmd(a, EliminateIfGuards(body), bodyPost)(s) == 
+                WpCmd(a, body, bodyPost)(s)
+      {
+        calc {
+          WpCmd(a, EliminateIfGuards(body), bodyPost)(s); { EliminateIfGuardsCorrect(a, body, s, bodyPost); }
+          WpCmd(a, body, bodyPost)(s);
+        }
+      }
+
+      ForallVarDeclsPointwise(a, varDecls, WpCmd(a, EliminateIfGuards(body), bodyPost), WpCmd(a, body, bodyPost), s);
+    case _ =>  //trivial (EliminateIfGuards is the identity function here)
+  }
+}
