util/SortUtil.dfy
@@ -1,0 +1,310 @@
+include "RustanMergeSort.dfy"
+
+module StringTO refines TotalOrder {
+  type T = string// the type to be compared
+  predicate method Leq(a: T, b: T) {
+    || a == []
+    || (b != [] && a[0] < b[0]) 
+    || (b != [] && a[0] == b[0] && Leq(a[1..], b[1..]))
+  } // Leq(a,b) iff a <= b
+  // Three properties of total orders.  Here, they are given as unproved
+  // lemmas, that is, as axioms.
+
+  lemma Antisymmetry ... { }
+  lemma Transitivity ... { }
+  lemma Totality ... { }
+}
+
+module StringMergeSort refines MergeSort {
+  import A = StringTO 
+}
+
+module SortUtil {
+  import StringTO
+  import StringMergeSort
+
+  lemma LexRelIsTotalOrder()
+  ensures IsTotalOrder(StringTO.Leq)
+  {
+    forall s1, s2
+    ensures StringTO.Leq(s1, s2) || StringTO.Leq(s2, s1)
+    { StringTO.Totality(s1, s2); }
+
+    forall s1, s2 | StringTO.Leq(s1, s2) && StringTO.Leq(s2, s1)
+    ensures s1 == s2
+    { StringTO.Antisymmetry(s1, s2); }
+
+    forall s1, s2, s3 | StringTO.Leq(s1, s2) && StringTO.Leq(s2, s3)
+    ensures StringTO.Leq(s1, s3)
+    { StringTO.Transitivity(s1, s2, s3); }
+  }
+
+  /** 
+  Various of the following definitions and lemmas are taken from http://leino.science/papers/krml275.html
+  */
+
+  predicate IsTotalOrder<A(!new)>(R: (A, A) -> bool) {
+    // connexity
+    && (forall a, b :: R(a, b) || R(b, a))
+    // antisymmetry
+    && (forall a, b :: R(a, b) && R(b, a) ==> a == b)
+    // transitivity
+    && (forall a, b, c :: R(a, b) && R(b, c) ==> R(a, c))
+  }
+
+  lemma ThereIsAMinimumGeneral<A>(R: (A, A) -> bool, s: set<A>)
+    requires s != {}
+    requires IsTotalOrder(R)
+    ensures exists x :: x in s && forall y | y in s :: R(x, y)
+  {
+    var x :| x in s;
+    if s == {x} {
+      // obviously, x is the minimum
+      assert x in s;
+      assert forall y | y in s :: x == y;
+    } else {
+      // The minimum in s might be x, or it might be the minimum
+      // in s - {x}. If we knew the minimum of the latter, then
+      // we could compare the two.
+      // Let's start by giving a name to the smaller set:
+      var s' := s - {x};
+      // So, s is the union of s' and {x}:
+      assert s == s' + {x};
+      // The following lemma call establishes that there is a
+      // minimum in s'.
+      ThereIsAMinimumGeneral(R, s');
+      var x' :| x' in s' && forall y | y in s' :: R(x', y);
+
+      var xMin := if R(x, x') then x else x';
+
+      assert xMin in s;
+
+      forall y | y in s
+      ensures R(xMin, y)
+      {
+      }
+    }
+  }
+
+  lemma ThereIsAMinimum(s: set<string>)
+    requires s != {}
+    ensures exists x :: x in s && forall y | y in s :: StringTO.Leq(x, y)
+  {
+    assert IsTotalOrder(StringTO.Leq) by {
+      LexRelIsTotalOrder();
+    }
+
+    ThereIsAMinimumGeneral(StringTO.Leq, s);
+  }  
+
+  predicate SortedSeq(a: seq<string>, low: int, high: int)
+    requires 0 <= low <= high <= |a|
+  {
+    forall i, j :: low <= i < j < high ==> StringTO.Leq(a[i], a[j])
+  }
+
+  lemma UniqueMinimum(x1: string, x2: string, s: set<string>)
+  requires x1 in s && x2 in s
+  requires forall x | x in s :: StringTO.Leq(x1,x)
+  requires forall x | x in s :: StringTO.Leq(x2,x)
+  ensures x1 == x2
+  {
+    assert StringTO.Leq(x1, x2) || StringTO.Leq(x2, x1) by {
+      StringTO.Totality(x1, x2);
+    }
+
+    if StringTO.Leq(x1, x2) && StringTO.Leq(x2, x1) {
+      assert x1 == x2 by {
+        StringTO.Antisymmetry(x1, x2);
+      }
+    }
+  }
+
+  lemma CardMono<A>(s1: set<A>, s2: set<A>)
+  requires s1 <= s2
+  ensures |s1| <= |s2|
+  {
+    if s1 == {} {
+
+    } else {
+      var x :| x in s1;
+      assert x in s2;
+
+      assert |s1-{x}| <= |s2-{x}| by {
+        CardMono(s1-{x}, s2-{x});
+      }
+    }
+  }
+
+  lemma CardSeqSet<A>(s: seq<A>)
+  ensures |s| >= |(set x | x in s)|
+  {
+    if |s| == 0 {
+
+    } else {
+      var xs := set x | x in s;
+      assert s[0] in xs;
+
+      var xs' := xs-{s[0]};
+
+      calc {
+        |s|;
+        |s[1..]|+1;
+      >= { CardSeqSet(s[1..]); }
+        |(set x | x in s[1..])|+1;
+      >=
+        { 
+          assert (set x | x in s[1..]) >= xs';
+          CardMono(xs', set x | x in s[1..]);
+        }
+        |xs'|+1;
+      }
+    }
+  }
+
+  lemma SortedUnique(s1: seq<string>, s2: seq<string>, xs: set<string>)
+    requires |s1| == |s2| == |xs|
+    requires (set x | x in s1) == (set x | x in s2) == xs
+    requires SortedSeq(s1, 0, |s1|)
+    requires SortedSeq(s2, 0, |s2|)
+    ensures s1 == s2
+  {
+    if xs == {} {
+    } else {
+      assert IsTotalOrder(StringTO.Leq) by {
+        LexRelIsTotalOrder();
+      }
+
+      assert forall y | y in xs :: StringTO.Leq(s1[0], y);
+      assert forall y | y in xs :: StringTO.Leq(s2[0], y);
+
+      assert s1[0] == s2[0] by {
+        UniqueMinimum(s1[0], s2[0], xs);
+      }
+
+      assert s1[1..] == s2[1..] by {
+        assert (set x | x in s1[1..]) + {s1[0]} == xs;
+        assert |s1[1..]| == |xs|-1;
+
+        if s1[0] in (set x | x in s1[1..]) {
+          assert (set x | x in s1[1..]) == xs;
+          assert |s1[1..]| >= |xs| by {
+            CardSeqSet(s1[1..]);
+          }
+          assert false;
+        }
+
+        if s2[0] in (set x | x in s2[1..]) {
+          assert (set x | x in s2[1..]) == xs;
+          assert |s2[1..]| >= |xs| by {
+            CardSeqSet(s2[1..]);
+          }
+          assert false;
+        }
+
+        SortedUnique(s1[1..], s2[1..], xs-{s1[0]});
+      }
+    }
+  }
+ 
+  lemma MultisetEmpty<A>(s: seq<A>)
+  requires multiset(s) == multiset{};
+  ensures s == []
+  {
+    if s != [] {
+      assert s[0] in multiset(s);
+      assert false;
+    } 
+  }
+
+  lemma MultisetNonempty<A>(s: seq<A>)
+  requires s != []
+  ensures multiset(s) != multiset{}
+  {
+    assert s[0] in multiset(s);
+  }
+  
+  lemma MultisetToSetSeq<A>(s1: seq<A>, s2: seq<A>)
+  requires multiset(s1) == multiset(s2)
+  ensures (set i | i in s1) == (set i | i in s2)
+  {
+    var s1Set := (set i | i in s1);
+    var s2Set := (set i | i in s2);
+
+    forall x | x in s1Set
+    ensures x in s2Set
+    {
+      assert x in multiset(s1);
+    }
+
+    forall x | x in s2Set
+    ensures x in s1Set
+    {
+      assert x in multiset(s2);
+    }
+  }
+
+  function SetToSequenceStr(s: set<string>) : seq<string>
+    ensures 
+      var res := SetToSequenceStr(s);
+      && (set x | x in res) == s
+      && |s| == |res|
+      && SortedSeq(res, 0, |res|)
+  {
+    if s == {} then
+      []
+    else
+      ThereIsAMinimum(s);
+      var min :| min in s && forall s' | s' in s :: StringTO.Leq(min, s');
+
+      assert {min}+(s-{min}) == s;
+
+      [min] + SetToSequenceStr(s-{min})
+  } by method {
+    var a: array<string> := new string[|s|];
+
+    var i := 0;
+    var s' := s;
+    while i < |s|
+      decreases s'
+      invariant |s'| == |s|-i
+      invariant 0 <= i <= |s|
+      invariant (set j | j in a[0..i]) == s-s'
+    {
+      var x :| x in s';
+
+      var a0Seq := a[..];
+
+      a[i] := x;
+
+      assert forall j | 0 <= j < i :: a[j] == a0Seq[j];
+      assert (set j | j in a[0..i]) == s-s';
+
+      var temp := s';
+      s' := s' - {x};
+
+      assert (set j | j in a[0..i+1]) == (s-temp)+{x};
+      i := i+1;
+    }
+
+    assert i == |s|;
+
+    assert (set j | j in a[0..i]) == s;
+    assert (set j | j in a[..]) == s;
+    var a0 := a[..];
+    
+    StringMergeSort.MergeSort(a);
+    
+    MultisetToSetSeq(a[..], a0);
+    
+    assert (set j | j in a[..]) == s;
+
+    var res := a[..];
+
+    assert res == SetToSequenceStr(s) by {
+      SortedUnique(res, SetToSequenceStr(s), s);
+    }
+
+    return res;
+  }
+}
